Tap

LogicalRefinement/Untyped/Basic.lean
@@ -78,7 +78,6 @@ inductive UntypedKind: List Nat -> Type
   -- Natural numbers
   | zero: UntypedKind []
   | succ: UntypedKind []
-  | natrec: UntypedKind [1, 0, 0, 2]
 
 inductive Untyped: Type
   | var (v: Nat)
@@ -94,7 +93,7 @@ inductive Untyped: Type
   | tri (k: UntypedKind [0, 0, 0]) (A: Untyped) (l: Untyped) (r: Untyped)
   -- TODO: no cases?
   | cases (k: UntypedKind [1, 0, 1, 1]) (K: Untyped) (d: Untyped) (l: Untyped) (r: Untyped)
-  | natrec (k: UntypedKind [1, 0, 0, 2]) (K: Untyped) (e: Untyped) (z: Untyped) (s: Untyped)
+  | natrec (K: Untyped) (e: Untyped) (z: Untyped) (s: Untyped)
 
 -- Types
 def Untyped.nats := const UntypedKind.nats
@@ -117,8 +116,6 @@ def Untyped.exists_ := abs UntypedKind.exists_
 def Untyped.eq := tri UntypedKind.eq
 
 -- Terms
-def Untyped.zero := const UntypedKind.zero
-def Untyped.succ := const UntypedKind.succ
 def Untyped.lam := abs UntypedKind.lam
 def Untyped.app := bin UntypedKind.app
 def Untyped.pair := bin UntypedKind.pair
@@ -149,6 +146,10 @@ def Untyped.wit := bin UntypedKind.wit
 def Untyped.let_wit := let_bin UntypedKind.let_wit
 def Untyped.refl := unary UntypedKind.refl
 
+-- Natural numbers
+def Untyped.zero := const UntypedKind.zero
+def Untyped.succ := const UntypedKind.succ
+
 @[simp] def Untyped.fv: Untyped -> Nat
   | var v => Nat.succ v
   | const c => 0
@@ -158,7 +159,7 @@ def Untyped.refl := unary UntypedKind.refl
   | abs _ A t => Nat.max (fv A) (fv t - 1)
   | tri _ A l r => Nat.max (fv A) (Nat.max (fv l) (fv r))
   | cases _ K d l r => Nat.max (fv K - 1) (Nat.max (fv d) (Nat.max (fv l - 1) (fv r - 1)))
-  | natrec _ K e z s => Nat.max (fv K - 1) (Nat.max (fv e) (Nat.max (fv z) (fv s - 2)))
+  | natrec K e z s => Nat.max (fv K - 1) (Nat.max (fv e) (Nat.max (fv z) (fv s - 2)))
 
 @[simp] def Untyped.has_dep: Untyped -> Nat -> Prop
   | var v, i => v = i
@@ -170,7 +171,7 @@ def Untyped.refl := unary UntypedKind.refl
   | tri _ A l r, i => has_dep A i ∨ has_dep l i ∨ has_dep r i
   | cases _ K d l r, i => 
     has_dep K (i + 1) ∨ has_dep d i ∨ has_dep l (i + 1) ∨ has_dep r (i + 1)
-  | natrec _ K e z s, i =>
+  | natrec K e z s, i =>
     has_dep K (i + 1) ∨ has_dep e i ∨ has_dep z i ∨ has_dep s (i + 2)
 
 theorem Untyped.has_dep_implies_fv (u: Untyped): {i: Nat} ->
