LogicalRefinement/Untyped/Wk.lean
@@ -12,8 +12,8 @@ import LogicalRefinement.Untyped.Basic
   | tri k A l r, ρ => tri k (A.wk ρ) (l.wk ρ) (r.wk ρ)
   | cases k K d l r, ρ => 
     cases k (K.wk ρ.lift) (d.wk ρ) (l.wk ρ.lift) (r.wk ρ.lift)
-  | natrec k K e z s, ρ =>
-    natrec k (K.wk ρ.lift) (e.wk ρ) (z.wk ρ) (s.wk (ρ.liftn 2))
+  | natrec K e z s, ρ =>
+    natrec (K.wk ρ.lift) (e.wk ρ) (z.wk ρ) (s.wk (ρ.liftn 2))
 
 @[simp] def Untyped.wk1 (u: Untyped) 
   := u.wk Wk.wk1
@@ -52,7 +52,7 @@ def Untyped.wknth_def {u: Untyped} {n}: u.wknth n = u.wk (Wk.wknth n) := rfl
     simp only [
       wk, IK (Wk.lift_equiv H), Id H, Il (Wk.lift_equiv H), Ir (Wk.lift_equiv H)
     ]
-  | natrec k K e z s IK Ie Iz Is =>
+  | natrec K e z s IK Ie Iz Is =>
     intros ρ σ H; 
     simp only [wk];
     simp only [
@@ -125,7 +125,7 @@ def Untyped.wk_bounds {u: Untyped}: {n m: Nat} -> {ρ: Wk} ->
           apply And.intro;
           case left => apply IHl (@Wk.liftn_maps ρ 1 n m Hm) Hl
           case right => apply IHr (@Wk.liftn_maps ρ 1 n m Hm) Hr
-    | natrec k K e z s IK Ie Iz Is =>
+    | natrec K e z s IK Ie Iz Is =>
       simp only [fv, Nat.max_r_le_split, Nat.le_sub_is_le_add]
       intros n m ρ Hm
       intro ⟨HK, He, Hz, Hs⟩
